code/rsapss/Hacl.RSAPSS.fst
@@ -29,14 +29,14 @@ let load_skey : RK.rsapss_load_skey_st t_limbs =
   RK.rsapss_load_skey RK.mk_runtime_rsapss_checks load_pkey
 
 
-val rsapss_sign: len:BN.meta_len t_limbs -> RI.rsapss_sign_st t_limbs (BE.mk_runtime_exp len).BE.mont.BM.bn.BN.len
-let rsapss_sign len a modBits eBits dBits skey sLen salt msgLen msg sgnt =
-  RI.rsapss_sign (BE.mk_runtime_exp len) a modBits eBits dBits skey sLen salt msgLen msg sgnt
+val rsapss_sign: RI.rsapss_sign_st t_limbs
+let rsapss_sign a modBits eBits dBits skey sLen salt msgLen msg sgnt =
+  RI.rsapss_sign a modBits eBits dBits skey sLen salt msgLen msg sgnt
 
 
-val rsapss_verify: len:BN.meta_len t_limbs -> RI.rsapss_verify_st t_limbs (BE.mk_runtime_exp len).BE.mont.BM.bn.BN.len
-let rsapss_verify len a modBits eBits pkey sLen k sgnt msgLen msg =
-  RI.rsapss_verify (BE.mk_runtime_exp len) a modBits eBits pkey sLen k sgnt msgLen msg
+val rsapss_verify: RI.rsapss_verify_st t_limbs
+let rsapss_verify a modBits eBits pkey sLen k sgnt msgLen msg =
+  RI.rsapss_verify a modBits eBits pkey sLen k sgnt msgLen msg
 
 
 val new_rsapss_load_pkey: RK.new_rsapss_load_pkey_st t_limbs
@@ -49,19 +49,11 @@ let new_rsapss_load_skey r modBits eBits dBits nb eb db =
   RK.new_rsapss_load_skey load_skey r modBits eBits dBits nb eb db
 
 
-val rsapss_skey_sign: len:BN.meta_len t_limbs -> RI.rsapss_skey_sign_st t_limbs (BE.mk_runtime_exp len).BE.mont.BM.bn.BN.len
-let rsapss_skey_sign len a modBits eBits dBits nb eb db sLen salt msgLen msg sgnt =
-  RI.rsapss_skey_sign
-    (BE.mk_runtime_exp len)
-    load_skey
-    (rsapss_sign len)
-    a modBits eBits dBits nb eb db sLen salt msgLen msg sgnt
+val rsapss_skey_sign: RI.rsapss_skey_sign_st t_limbs
+let rsapss_skey_sign a modBits eBits dBits nb eb db sLen salt msgLen msg sgnt =
+  RI.rsapss_skey_sign load_skey rsapss_sign a modBits eBits dBits nb eb db sLen salt msgLen msg sgnt
 
 
-val rsapss_pkey_verify: len:BN.meta_len t_limbs -> RI.rsapss_pkey_verify_st t_limbs (BE.mk_runtime_exp len).BE.mont.BM.bn.BN.len
-let rsapss_pkey_verify len a modBits eBits nb eb sLen k sgnt msgLen msg =
-  RI.rsapss_pkey_verify
-    (BE.mk_runtime_exp len)
-    load_pkey
-    (rsapss_verify len)
-     a modBits eBits nb eb sLen k sgnt msgLen msg
+val rsapss_pkey_verify: RI.rsapss_pkey_verify_st t_limbs
+let rsapss_pkey_verify a modBits eBits nb eb sLen k sgnt msgLen msg =
+  RI.rsapss_pkey_verify load_pkey rsapss_verify a modBits eBits nb eb sLen k sgnt msgLen msg
